WIP - progress on removing manual labour

Risc0/Basic.lean
@@ -59,6 +59,9 @@ def copyLast (buf : Buffer) : Buffer :=
 def get! (buf : Buffer) (idx : Idx) : Option Felt :=
   List.get! (List.get! buf idx.time) idx.data
 
+-- @[simp]
+-- lemma www : buffer.get! [[some ...]] (0...k)
+
 def getBufferAtTime! (buf : Buffer) (timeIdx : ℕ) : BufferAtTime :=
   List.get! buf timeIdx
 
@@ -220,11 +223,44 @@ def update (state : State) (name : String) (x : Option Lit) : State :=
               else {state with isFailed := true}
             | .none        => {state with isFailed := true}
 
-def updateFelts (state : State) (name : String) (x : Felt) : State :=
-  { state with felts := state.felts[⟨name⟩] ←ₘ x }
+def updateFelts (state : State) (name : FeltVar) (x : Felt) : State :=
+  { state with felts := state.felts[name] ←ₘ x }
 
 lemma updateFelts_def : 
-  updateFelts st k v = { st with felts := st.felts[⟨k⟩] ←ₘ v } := rfl
+  updateFelts st k v = { st with felts := st.felts[k] ←ₘ v } := rfl
+
+@[simp]
+lemma updateFelts_felts_get {st : State} {name : FeltVar} {x : Felt} :
+  (updateFelts st name x).felts[name]! = some x := by
+  simp [updateFelts, Map.update_def, getElem!]
+
+-- This simp lemma feels bad with name ≠ name' but somehow it works out in our context.
+@[simp]
+lemma updateFelts_felts_get_ne {st : State} {name name' : FeltVar} {x : Felt}
+  (h : name ≠ name') : (updateFelts st name x).felts[name']! = st.felts[name']! := by
+  simp [updateFelts, Map.update_def, getElem!]
+  aesop
+
+@[simp]
+lemma updateFelts_buffers : (updateFelts st name x).buffers = st.buffers := by simp [updateFelts]
+
+@[simp]
+lemma updateFelts_bufferWidths : (updateFelts st name x).bufferWidths = st.bufferWidths := by simp [updateFelts]
+
+@[simp]
+lemma updateFelts_constraints : (updateFelts st name x).constraints = st.constraints := by simp [updateFelts]
+
+@[simp]
+lemma updateFelts_cycle : (updateFelts st name x).cycle = st.cycle := by simp [updateFelts]
+
+@[simp]
+lemma updateFelts_isFailed : (updateFelts st name x).isFailed = st.isFailed := by simp [updateFelts]
+
+@[simp]
+lemma updateFelts_props : (updateFelts st name x).props = st.props := by simp [updateFelts]
+
+@[simp]
+lemma updateFelts_vars : (updateFelts st name x).vars = st.vars := by simp [updateFelts]
 
 -- @[simp]
 lemma update_val {state : State} {name : String} {x : Felt} :
@@ -232,7 +268,7 @@ lemma update_val {state : State} {name : String} {x : Felt} :
 
 @[simp]
 lemma update_val' {state : State} {name : String} {x : Felt} :
-  update state name (.some (.Val x)) = state.updateFelts name x := rfl
+  update state name (.some (.Val x)) = state.updateFelts ⟨name⟩ x := rfl
 
 @[simp]
 lemma update_constraint {state : State} {name : String} {c : Prop} :
@@ -274,6 +310,14 @@ end State
 instance : Inhabited State := ⟨State.init_default 42 42⟩
 
 notation:61 st "[" n:61 "]" " ←ₛ " x:49 => State.update st n x
+
+namespace State
+
+-- @[simp]
+-- lemma set_felts {st : State} {name : String} {x} :
+--   (st[name] ←ₛ some (Lit.Val x)).felts = _ := _
+
+end State
 
 inductive IsNondet :=
   | InNondet
@@ -354,43 +398,43 @@ def rowColOfWidthIdx (width idx : ℕ) : Back × ℕ := (idx / width, idx % widt
 
 lemma col_lt_width (h : 0 < width) : (rowColOfWidthIdx width idx).2 < width := Nat.mod_lt _ h
 
+abbrev Buffer.back (st : State) (buf : BufferVar) (back : Back) (offset : ℕ) :=
+  st.buffers[buf].get!.get! (st.cycle - back.toNat, offset)
+
+abbrev isGetValid (st : State) (buf : BufferVar) (back : Back) (offset : ℕ) :=
+  back ≤ st.cycle ∧
+  buf ∈ st.vars ∧
+  offset < st.bufferWidths.get! buf ∧
+  (Buffer.back st buf back offset).isSome
+
 -- Evaluate a pure functional circuit.
 def Op.eval {x} (st : State) (op : Op x) : Option Lit :=
   match op with
     -- Constants
     | Const const => .some <| .Val const
     -- Arith
-    | Add lhs rhs => .some <| .Val <| (st.felts lhs).get! + (st.felts rhs).get!
-    | Sub lhs rhs => .some <| .Val <| (st.felts lhs).get! - (st.felts rhs).get!
-    | Neg lhs     => .some <| .Val <| 0                   - (st.felts lhs).get!
-    | Mul lhs rhs => .some <| .Val <| (st.felts lhs).get! * (st.felts rhs).get!
-    | Pow lhs rhs => .some <| .Val <| (st.felts lhs).get! ^ rhs
-    | Inv x => .some <| .Val <|
-                 match st.felts x with
-                   | some x => if x = 0 then 0 else x⁻¹
-                   | _      => default
+    | Add lhs rhs => .some <| .Val <| st.felts[lhs].get! + st.felts[rhs].get!
+    | Sub lhs rhs => .some <| .Val <| st.felts[lhs].get! - st.felts[rhs].get!
+    | Neg lhs     => .some <| .Val <| 0                  - st.felts[lhs].get!
+    | Mul lhs rhs => .some <| .Val <| st.felts[lhs].get! * st.felts[rhs].get!
+    | Pow lhs rhs => .some <| .Val <| st.felts[lhs].get! ^ rhs
+    | Inv x => .some <| .Val <| if st.felts[x]!.get! = 0 then 0 else st.felts[x]!.get!⁻¹
     -- Logic
-    | Isz x => .some <| .Val <| if (st.felts x).get! = 0 then 1 else 0
+    | Isz x => .some <| .Val <| if st.felts[x]!.get! = 0 then 1 else 0
     -- Constraints
-    | AndEqz c val           => .some <| .Constraint <| (st.props c).get! ∧ (st.felts val).get! = 0
+    | AndEqz c val           => .some <| .Constraint <| st.props[c].get! ∧ st.felts[val].get! = 0
     | AndCond old cond inner =>
-        .some <| .Constraint <|
-          (st.props old).get! ∧
-            if (st.felts cond).get! = 0
-            then _root_.True
-            else (st.props inner).get!
+        .some <| .Constraint <| st.props[old].get! ∧
+                                if st.felts[cond].get! = 0
+                                then _root_.True
+                                else st.props[inner].get!
     | True                   => .some <| .Constraint _root_.True
     -- Buffers
     | Alloc size          => .some <| .Buf <| List.replicate size .none
-    | Back buf back       => .some <| .Buf <| (List.get! (st.buffers.get! buf) st.cycle).slice 0 back
-    | Get buf back offset => let val := (st.buffers.get! buf).get! ((st.cycle - back.toNat), offset)
-                              if
-                                back ≤ st.cycle ∧
-                                buf ∈ st.vars ∧
-                                offset < st.bufferWidths.get! buf ∧
-                                val.isSome
-                              then .some <| .Val val.get!
-                              else .none
+    | Back buf back       => .some <| .Buf <| st.buffers[buf].get![st.cycle]!.slice 0 back
+    | Get buf back offset => if isGetValid st buf back offset
+                             then .some <| .Val (Buffer.back st buf back offset).get!
+                             else .none
     | GetGlobal buf offset => if buf ∈ st.vars
                               then
                                 let buffer := st.buffers.get! buf
@@ -442,9 +486,7 @@ lemma eval_mul : Γ st ⟦@Mul α x y⟧ₑ = .some (.Val ((st.felts x).get! * (
 lemma eval_isz : Γ st ⟦??₀x⟧ₑ = .some (.Val (if (st.felts x).get! = 0 then 1 else 0)) := rfl
 
 @[simp]
-lemma eval_inv : Γ st ⟦Inv x⟧ₑ = .some (.Val (match st.felts x with
-                                               | some x => if x = 0 then 0 else x⁻¹
-                                               | _      => default)) := rfl
+lemma eval_inv : Γ st ⟦Inv x⟧ₑ = .some (.Val (if st.felts[x]!.get! = 0 then 0 else st.felts[x]!.get!⁻¹)) := rfl
 
 @[simp]
 lemma eval_andEqz : Γ st ⟦@AndEqz α c x⟧ₑ =
@@ -502,6 +544,12 @@ def State.setBufferElementImpl (st : State) (bufferVar : BufferVar) (idx: Buffer
 def State.set! (st : State) (bufferVar : BufferVar) (offset : ℕ) (val : Felt) : State :=
   st.setBufferElementImpl bufferVar (((st.buffers.get! bufferVar).length - 1), offset) val
 
+@[simp]
+lemma State.set!_felts {st : State} {bufferVar : BufferVar} {offset : ℕ} {val : Felt} :
+  (State.set! st bufferVar offset val).felts = st.felts := by
+  unfold set! setBufferElementImpl
+  aesop
+
 def State.setGlobal! (st : State) (bufferVar : BufferVar) (offset : ℕ) (val : Felt) : State :=
   let width := st.bufferWidths.get! bufferVar
   st.setBufferElementImpl bufferVar (Buffer.Idx.from1D offset width) val
@@ -513,26 +561,15 @@ def MLIR.run {α : IsNondet} (program : MLIR α) (st : State) : State :=
   match program with
     -- Meta
     | Assign name op => st[name] ←ₛ Γ st ⟦op⟧ₑ
-    | Eqz x =>
-        match st.felts x with
-          | .some x => withEqZero x st
-          | _       => st
-    | If x program => 
-        match st.felts x with
-          | .some x => if x = 0 then st else program.run st
-          | _       => st
-    | Nondet block => block.run st
-    | Sequence a b => b.run (a.run st)
+    | Eqz x          => withEqZero st.felts[x]!.get! st
+    | If x program   => if st.felts[x]!.get! = 0 then st else program.run st
+    | Nondet block   => block.run st
+    | Sequence a b   => b.run (a.run st)
     -- Ops
-    | Fail => {st with isFailed := true}
-    | Set buf offset val =>
-        match st.felts val with
-          | .some val => st.set! buf offset val
-          | _         => st
-    | SetGlobal buf offset val =>
-        match st.felts val with
-          | .some val => st.setGlobal! buf offset val -- Behind the scenes setGlobal actually flattens a 2d buffer into a 1d buffer
-          | _         => st                           -- and indexes into it. This is a side effect of global buffers only being 1d anyway
+    | Fail                     => {st with isFailed := true}
+    | Set buf offset val       => st.set! buf offset st.felts[val]!.get!
+    | SetGlobal buf offset val => st.setGlobal! buf offset st.felts[val]!.get! -- Behind the scenes setGlobal actually flattens a 2d buffer into a 1d buffer
+                                                                               -- and indexes into it. This is a side effect of global buffers only being 1d anyway
 
 @[simp]
 abbrev MLIR.runProgram (program : MLIRProgram) := program.run
